tarjan directed low invariant proofs and plans

SeparationLogic/algorithms/Tarjan_directed/Tarjan_scc_is_low.v
@@ -256,6 +256,43 @@ Section IS_LOW.
   Definition RootFinal (u: V) (s: St): Prop :=
     RootAfterMaybePop u s.
 
+  Definition ChildNoActiveTarget (v: V) (s: St): Prop :=
+    forall x b,
+      dg_reachable (state_to_dfs_tree g s root) v x ->
+      Edge x b ->
+      Active b s ->
+      ~ tree_edge s x b ->
+      False.
+
+  Definition ChildLowContribution (u v: V) (s: St): Prop :=
+    (Active v s /\ LoopCoreShape v (edge_set v) s /\ RootLowCorrect v s) \/
+    (~ Active v s /\ low s v = dfn s v /\
+     dfn s u < dfn s v /\ ChildNoActiveTarget v s).
+
+  Definition ParentLowFrame
+             (u: V) (done: V -> Prop) (s_before s_after: St): Prop :=
+    low s_after u = low s_before u /\
+    (forall b,
+      PartialLowCandidate u done s_before b ->
+      PartialLowCandidate u done s_after b /\
+      dfn s_after b = dfn s_before b) /\
+    (forall b,
+      PartialLowCandidate u done s_after b ->
+      PartialLowCandidate u done s_before b /\
+      dfn s_after b = dfn s_before b).
+
+  Definition ChildContributionContract
+             (u v: V) (done: V -> Prop) (s_before s_after: St): Prop :=
+    ParentLowFrame u done s_before s_after /\
+    LoopCoreShape u (done_after done v) s_after /\
+    LoopAuxFacts u s_after /\
+    Closed s_after /\
+    TreeEdgesAreGraphEdges s_after /\
+    Visited v s_after /\
+    fa s_after v = u /\
+    fa s_after v <> v /\
+    ChildLowContribution u v s_after.
+
   Lemma done_after_intro_old (done: V -> Prop) (a b: V):
     done b -> done_after done a b.
   Proof.
@@ -266,6 +303,15 @@ Section IS_LOW.
     done_after done a a.
   Proof.
     unfold done_after. sets_unfold. auto.
+  Qed.
+
+  Lemma done_after_elim (done: V -> Prop) (a b: V):
+    done_after done a b -> done b \/ b = a.
+  Proof.
+    unfold done_after. sets_unfold.
+    intros [Hdone | Heq].
+    - left. exact Hdone.
+    - right. symmetry. exact Heq.
   Qed.
 
   Lemma partial_tree_done_mono (u a x: V) (done: V -> Prop) (s: St):
@@ -365,6 +411,114 @@ Section IS_LOW.
   Proof.
     unfold LowComplete. intros H b Ht.
     apply H. apply partial_low_candidate_done_mono. exact Ht.
+  Qed.
+
+  Lemma processed_tree_child_done_equiv
+        (u: V) (done1 done2: V -> Prop) (s: St):
+    done1 == done2 ->
+    ProcessedTreeChild u done1 s ->
+    ProcessedTreeChild u done2 s.
+  Proof.
+    intros Hdone Hprocessed child Hchild_vis Hfa Hfane.
+    sets_unfold in Hdone.
+    apply Hdone.
+    exact (Hprocessed child Hchild_vis Hfa Hfane).
+  Qed.
+
+  Lemma loop_core_shape_done_equiv
+        (u: V) (done1 done2: V -> Prop) (s: St):
+    done1 == done2 ->
+    LoopCoreShape u done1 s ->
+    LoopCoreShape u done2 s.
+  Proof.
+    intros Hdone [Hwf [Htree [Huvis [Hdone_edge [Hdone_vis Hprocessed]]]]].
+    sets_unfold in Hdone.
+    split; [exact Hwf |].
+    split; [exact Htree |].
+    split; [exact Huvis |].
+    split.
+    - intros a Ha. apply Hdone_edge. apply Hdone. exact Ha.
+    - split.
+      + intros a Ha. apply Hdone_vis. apply Hdone. exact Ha.
+      + unfold ProcessedTreeChild in *.
+        intros child Hchild_vis Hfa Hfane.
+        apply Hdone.
+        exact (Hprocessed child Hchild_vis Hfa Hfane).
+  Qed.
+
+  Lemma partial_active_target_done_equiv
+        (u b: V) (done1 done2: V -> Prop) (s: St):
+    done1 == done2 ->
+    PartialActiveTarget u done1 s b ->
+    PartialActiveTarget u done2 s b.
+  Proof.
+    intros Hdone Htarget.
+    sets_unfold in Hdone.
+    unfold PartialActiveTarget in Htarget |- *.
+    destruct Htarget as [Hdirect | Hchild].
+    - destruct Hdirect as [a [Hdone_a [Hb [Hedge [Hactive Hnot_tree]]]]].
+      left. exists a. repeat split; auto.
+      apply Hdone. exact Hdone_a.
+    - destruct Hchild as
+        [child [x [Hdone_child [Hedge [Hfa [Hfane [Hreach [Hxb [Hactive Hnot_tree]]]]]]]]].
+      right. exists child, x. repeat split; auto.
+      apply Hdone. exact Hdone_child.
+  Qed.
+
+  Lemma partial_low_candidate_done_equiv
+        (u b: V) (done1 done2: V -> Prop) (s: St):
+    done1 == done2 ->
+    PartialLowCandidate u done1 s b ->
+    PartialLowCandidate u done2 s b.
+  Proof.
+    intros Hdone Hcandidate.
+    unfold PartialLowCandidate in Hcandidate |- *.
+    destruct Hcandidate as [Hb | Htarget].
+    - left. exact Hb.
+    - right.
+      eapply partial_active_target_done_equiv; eauto.
+  Qed.
+
+  Lemma low_correct_done_equiv
+        (u: V) (done1 done2: V -> Prop) (s: St):
+    done1 == done2 ->
+    LowCorrect u done1 s ->
+    LowCorrect u done2 s.
+  Proof.
+    intros Hdone [Hsound Hcomplete]. split.
+    - destruct Hsound as [witness [Hcandidate Hlow]].
+      exists witness. split.
+      + eapply partial_low_candidate_done_equiv; eauto.
+      + exact Hlow.
+    - intros target Hcandidate.
+      apply Hcomplete.
+      eapply partial_low_candidate_done_equiv.
+      + symmetry. exact Hdone.
+      + exact Hcandidate.
+  Qed.
+
+  Lemma loop_core_inv_done_equiv
+        (u: V) (done1 done2: V -> Prop) (s: St):
+    done1 == done2 ->
+    LoopCoreInv u done1 s ->
+    LoopCoreInv u done2 s.
+  Proof.
+    intros Hdone [Hshape [Hclosed Hlow]].
+    split.
+    - eapply loop_core_shape_done_equiv; eauto.
+    - split; [exact Hclosed |].
+      eapply low_correct_done_equiv; eauto.
+  Qed.
+
+  Lemma loop_inv_done_equiv
+        (u: V) (done1 done2: V -> Prop) (s: St):
+    done1 == done2 ->
+    LoopInv u done1 s ->
+    LoopInv u done2 s.
+  Proof.
+    intros Hdone [Haux Hcore].
+    split; [exact Haux |].
+    eapply loop_core_inv_done_equiv; eauto.
   Qed.
 
   (** Preloop **)
@@ -661,6 +815,39 @@ Section IS_LOW.
     unfold update_low. unfold_op. intro_state. hoare_auto_s.
     - subst s. simpl. exact H.
     - destruct H1 as [Heq _]. subst s. exact H.
+  Qed.
+
+  Lemma set_fa_preserves_stack_nodup (v p: V):
+    Hoare (StackNoDup)
+          (set_fa v p)
+          (fun _ s => StackNoDup s).
+  Proof.
+    unfold set_fa. intro_state. hoare_auto_s.
+    subst s. simpl. exact H.
+  Qed.
+
+  Lemma get_low_update_low_preserves_stack_nodup (u v: V):
+    Hoare (StackNoDup)
+          (lv <- get' (fun s => low s v);; update_low u lv)
+          (fun _ s => StackNoDup s).
+  Proof.
+    intro_state.
+    eapply Hoare_bind. { eapply Hoare_get'. } simpl. intros lv.
+    eapply Hoare_conseq_pre.
+    2: apply update_low_preserves_stack_nodup.
+    intros s1 Hs1. destruct Hs1. subst s1. exact H.
+  Qed.
+
+  Lemma get_dfn_update_low_preserves_stack_nodup (u v: V):
+    Hoare (StackNoDup)
+          (dv <- get' (fun s => dfn s v);; update_low u dv)
+          (fun _ s => StackNoDup s).
+  Proof.
+    intro_state.
+    eapply Hoare_bind. { eapply Hoare_get'. } simpl. intros dv.
+    eapply Hoare_conseq_pre.
+    2: apply update_low_preserves_stack_nodup.
+    intros s1 Hs1. destruct Hs1. subst s1. exact H.
   Qed.
 
   Lemma update_low_preserves_loop_core_shape
@@ -1059,6 +1246,130 @@ Section IS_LOW.
              (conj Hclosed Hlow)).
   Qed.
 
+  Lemma set_fa_pending_preserves_loop_aux_facts
+        (u v: V):
+    Hoare
+      (LoopAuxFacts u)
+      (set_fa v u)
+      (fun _ s => LoopAuxFacts u s).
+  Proof.
+    unfold LoopAuxFacts, OrderFacts.
+    apply Hoare_conj with
+      (Q1 := fun _ s => NoUnvisitedReach s).
+    { eapply Hoare_conseq_pre.
+      2: apply set_fa_keep_settled_closed.
+      intros s [Hsettled _]. exact Hsettled. }
+    apply Hoare_conj with
+      (Q1 := fun _ s => Active u s).
+    { eapply Hoare_conseq_pre.
+      2: apply (set_fa_keep_in_stack v u u).
+      intros s [_ [Hactive _]]. exact Hactive. }
+    apply Hoare_conj with
+      (Q1 := fun _ s => stack_dfn_order s).
+    { eapply Hoare_conseq_pre.
+      2: apply set_fa_keep_stack_dfn_order.
+      intros s [_ [_ [Hstack_order _]]]. exact Hstack_order. }
+    apply Hoare_conj with
+      (Q1 := fun _ s => dfn_injective s).
+    { eapply Hoare_conseq_pre.
+      2: apply set_fa_keep_dfn_injective.
+      intros s [_ [_ [_ [Hinj _]]]]. exact Hinj. }
+    { unfold set_fa. intro_state. hoare_auto_s.
+      subst s. simpl.
+      destruct H as [_ [_ [_ [_ Hnodup]]]]. exact Hnodup. }
+  Qed.
+
+  Lemma set_fa_pending_preserves_parent_loop
+        (u v: V) (done: V -> Prop):
+    Hoare
+      (fun s: St =>
+         LoopInv u done s /\
+         Edge u v /\
+         ~ Visited v s)
+      (set_fa v u)
+      (fun _ s => LoopInv u done s).
+  Proof.
+    unfold LoopInv.
+    apply Hoare_conj with
+      (Q1 := fun _ s => LoopAuxFacts u s).
+    { eapply Hoare_conseq_pre.
+      2: apply set_fa_pending_preserves_loop_aux_facts.
+      intros s [[Haux _] _]. exact Haux. }
+    { eapply Hoare_conseq_pre.
+      2: apply set_fa_pending_preserves_parent_core.
+      intros s [[Haux Hcore] [Hedge Hnotvis]].
+      destruct Haux as [_ [Hactive _]].
+      exact (conj Hcore (conj Hedge (conj Hactive Hnotvis))). }
+  Qed.
+
+  Lemma set_fa_pending_prepares_child_entry
+        (u v: V) (done: V -> Prop):
+    Hoare
+      (fun s: St =>
+         LoopInv u done s /\
+         Edge u v /\
+         ~ Visited v s)
+      (set_fa v u)
+      (fun _ s =>
+         LoopInv u done s /\
+         EntryPre v s /\
+         fa s v = u /\
+         fa s v <> v).
+  Proof.
+    unfold set_fa. intro_state. hoare_auto_s.
+    subst s. change
+      (LoopInv u done (set_fa_state s0 v u) /\
+       EntryPre v (set_fa_state s0 v u) /\
+       fa (set_fa_state s0 v u) v = u /\
+       fa (set_fa_state s0 v u) v <> v).
+    destruct H as [Hinv [Hedge Hnotvis]].
+    destruct Hinv as [Haux Hcore].
+    destruct Hcore as [Hshape [Hclosed Hlow]].
+    destruct Hshape as
+      [Hwf [Htree_sound [Huvis [Hdone_edge [Hdone_vis Hprocessed]]]]].
+    destruct Haux as [Hsettled [Hactive Horder]].
+    assert (Hloop_post: LoopInv u done (set_fa_state s0 v u)).
+    { unfold LoopInv. split.
+      - unfold LoopAuxFacts, OrderFacts in *.
+        simpl. exact (conj Hsettled (conj Hactive Horder)).
+      - apply set_fa_pending_preserves_loop_core_inv; auto.
+        exact (conj
+                 (conj Hwf
+                   (conj Htree_sound
+                     (conj Huvis
+                       (conj Hdone_edge
+                         (conj Hdone_vis Hprocessed)))))
+                 (conj Hclosed Hlow)). }
+    assert (Hfa_new: fa (set_fa_state s0 v u) v = u).
+    { unfold set_fa_state. simpl. unfold equiv_decb.
+      destruct (equiv_dec v v) as [_ | Hneq].
+      - reflexivity.
+      - exfalso. apply Hneq. reflexivity. }
+    assert (Hu_ne_v: u <> v).
+    { intros Hu_eq_v. apply Hnotvis. rewrite <- Hu_eq_v. exact Huvis. }
+    assert (Hfa_ne: fa (set_fa_state s0 v u) v <> v).
+    { rewrite Hfa_new. exact Hu_ne_v. }
+    assert (Hentry: EntryPre v (set_fa_state s0 v u)).
+    { assert (Hwf_pre: wf_scc_state_pre g root v (set_fa_state s0 v u)).
+      { exact (conj
+                 (set_fa_pending_preserves_wf_scc_state s0 u v Hwf Huvis Hnotvis)
+                 Hnotvis). }
+      assert (Hclosed_post: Closed (set_fa_state s0 v u)).
+      { apply set_fa_pending_preserves_closed. exact Hclosed. }
+      assert (Htree_post: TreeEdgesAreGraphEdges (set_fa_state s0 v u)).
+      { apply set_fa_pending_preserves_tree_edges_are_graph_edges; auto. }
+      assert (Hincoming:
+                fa (set_fa_state s0 v u) v <> v ->
+                Edge (fa (set_fa_state s0 v u) v) v).
+      { intros _. rewrite Hfa_new. exact Hedge. }
+      exact (conj Hwf_pre
+              (conj Hsettled
+                (conj Hclosed_post
+                  (conj Htree_post
+                    (conj Horder Hincoming))))). }
+    exact (conj Hloop_post (conj Hentry (conj Hfa_new Hfa_ne))).
+  Qed.
+
   Lemma current_active_edge_not_tree
         (u v: V) (done: V -> Prop) (s: St):
     LoopInv u done s ->
@@ -1083,4 +1394,959 @@ Section IS_LOW.
     rewrite Hsnd_child.
     exact (Hprocessed child Hchild_vis Hfa_child Hfane).
   Qed.
+
+  Lemma loop_core_shape_done_after_active
+        (u v: V) (done: V -> Prop) (s: St):
+    LoopCoreShape u done s ->
+    Edge u v ->
+    Visited v s ->
+    LoopCoreShape u (done_after done v) s.
+  Proof.
+    intros [Hwf [Htree [Huvis [Hdone_edge [Hdone_vis Hprocessed]]]]]
+           Hedge Hvis.
+    assert (Hdone_edge_after:
+              forall a, done_after done v a -> Edge u a).
+    { intros a Hdone_after.
+      destruct (done_after_elim done v a Hdone_after) as [Hdone | Ha_eq_v].
+      + apply Hdone_edge. exact Hdone.
+      + subst a. exact Hedge. }
+    assert (Hdone_vis_after:
+              forall a, done_after done v a -> Visited a s).
+    { intros a Hdone_after.
+      destruct (done_after_elim done v a Hdone_after) as [Hdone | Ha_eq_v].
+      + apply Hdone_vis. exact Hdone.
+      + subst a. exact Hvis. }
+    assert (Hprocessed_after: ProcessedTreeChild u (done_after done v) s).
+    { unfold ProcessedTreeChild in *.
+      intros child Hchild_vis Hfa Hfane.
+      apply done_after_intro_old.
+      exact (Hprocessed child Hchild_vis Hfa Hfane). }
+    exact (conj Hwf
+            (conj Htree
+              (conj Huvis
+                (conj Hdone_edge_after
+                  (conj Hdone_vis_after Hprocessed_after))))).
+  Qed.
+
+  Lemma partial_low_candidate_active_done_after_cases
+        (u v b: V) (done: V -> Prop) (s: St):
+    LoopCoreShape u done s ->
+    ~ done v ->
+    Visited v s ->
+    PartialLowCandidate u (done_after done v) s b ->
+    PartialLowCandidate u done s b \/ b = v.
+  Proof.
+    intros Hshape Hnot_done Hvis Hcandidate.
+    destruct Hshape as [_ [_ [_ [_ [_ Hprocessed]]]]].
+    unfold PartialLowCandidate in Hcandidate |- *.
+    destruct Hcandidate as [Hb_root | Htarget].
+    - left. left. exact Hb_root.
+    - unfold PartialActiveTarget in Htarget.
+      destruct Htarget as [Hdirect | Hchild].
+      + destruct Hdirect as [a [Hdone_after [Hb [Hedge [Hactive Hnot_tree]]]]].
+        destruct (done_after_elim done v a Hdone_after) as [Hdone | Ha_eq_v].
+        * left. right. left.
+          exists a. repeat split; auto.
+        * right. rewrite Hb. exact Ha_eq_v.
+      + destruct Hchild as
+          [child [x [Hdone_after [Hedge [Hfa [Hfane [Hreach [Hxb [Hactive Hnot_tree]]]]]]]]].
+        destruct (done_after_elim done v child Hdone_after) as [Hdone | Hchild_eq_v].
+        * left. right. right.
+          exists child, x. repeat split; auto.
+        * exfalso. apply Hnot_done.
+          rewrite Hchild_eq_v in Hfa, Hfane.
+          exact (Hprocessed v Hvis Hfa Hfane).
+  Qed.
+
+  Lemma update_low_active_direct_preserves_loop_core_shape
+        (u v: V) (done: V -> Prop) (n: nat):
+    Hoare
+      (fun s: St => LoopCoreShape u done s /\ Edge u v /\ Visited v s)
+      (update_low u n)
+      (fun _ s => LoopCoreShape u (done_after done v) s).
+  Proof.
+    eapply Hoare_conseq_post.
+    2: {
+      apply Hoare_conj with
+        (Q1 := fun _ s => LoopCoreShape u done s)
+        (Q2 := fun _ s => Edge u v /\ Visited v s).
+      - eapply Hoare_conseq_pre.
+        2: apply update_low_preserves_loop_core_shape.
+        intros s [Hshape _].
+        assert (Huvis: u ∈ visited s).
+        { destruct Hshape as [_ [_ [Huvis _]]]. exact Huvis. }
+        exact (conj Hshape Huvis).
+      - apply Hoare_conj with
+          (Q1 := fun _ _ => Edge u v)
+          (Q2 := fun _ s => Visited v s).
+        + unfold update_low. unfold_op. intro_state. hoare_auto_s;
+            try (destruct H as [_ [Hedge _]]; exact Hedge);
+            try (destruct H1 as [_ _];
+                 destruct H as [_ [Hedge _]]; exact Hedge).
+        + eapply Hoare_conseq_pre.
+          2: apply (update_low_keep_visited u v n).
+          intros s [_ [_ Hvis]]. exact Hvis. }
+    intros _ s [Hshape [Hedge Hvis]].
+    apply loop_core_shape_done_after_active; auto.
+  Qed.
+
+  Lemma update_low_active_direct_preserves_low_correct
+        (u v: V) (done: V -> Prop) (n: nat):
+    Hoare
+      (fun s: St =>
+         LoopCoreShape u done s /\
+         LowCorrect u done s /\
+         Edge u v /\
+         ~ done v /\
+         Visited v s /\
+         Active v s /\
+         ~ tree_edge s u v /\
+         n = dfn s v)
+      (update_low u n)
+      (fun _ s => LowCorrect u (done_after done v) s).
+  Proof.
+    unfold update_low. unfold_op. intro_state. hoare_auto_s.
+    - subst s. simpl.
+      destruct H as [Hshape [[Hsound Hcomplete]
+        [Hedge [Hnot_done [Hvis [Hactive [Hnot_tree Hn]]]]]]].
+      split.
+      + exists v. split.
+        * apply partial_low_candidate_direct_active; auto.
+        * simpl. unfold equiv_decb.
+          destruct (equiv_dec u u) as [_ | Hneq].
+          -- exact Hn.
+          -- exfalso. apply Hneq. reflexivity.
+      + intros target Hcandidate.
+        pose proof (partial_low_candidate_active_done_after_cases
+                      u v target done s0 Hshape Hnot_done Hvis Hcandidate)
+          as [Hold_candidate | Hb_eq_v].
+        * specialize (Hcomplete target Hold_candidate).
+          simpl. unfold equiv_decb.
+          destruct (equiv_dec u u) as [_ | Hneq].
+          -- lia.
+          -- exfalso. apply Hneq. reflexivity.
+        * subst target.
+          simpl. unfold equiv_decb.
+          destruct (equiv_dec u u) as [_ | Hneq].
+          -- lia.
+          -- exfalso. apply Hneq. reflexivity.
+    - destruct H1 as [Heq Hnot_lt]. subst s.
+      destruct H as [Hshape [[Hsound Hcomplete]
+        [Hedge [Hnot_done [Hvis [Hactive [Hnot_tree Hn]]]]]]].
+      split.
+      + destruct Hsound as [witness [Hcandidate Hlow]].
+        exists witness. split.
+        * apply partial_low_candidate_done_mono. exact Hcandidate.
+        * exact Hlow.
+      + intros target Hcandidate.
+        pose proof (partial_low_candidate_active_done_after_cases
+                      u v target done s0 Hshape Hnot_done Hvis Hcandidate)
+          as [Hold_candidate | Hb_eq_v].
+        * apply Hcomplete. exact Hold_candidate.
+        * subst target. rewrite Hn in Hnot_lt. lia.
+  Qed.
+
+  Lemma update_low_active_direct_preserves_loop_inv
+        (u v: V) (done: V -> Prop) (n: nat):
+    Hoare
+      (fun s: St =>
+         LoopInv u done s /\
+         Edge u v /\
+         ~ done v /\
+         Visited v s /\
+         Active v s /\
+         ~ tree_edge s u v /\
+         n = dfn s v)
+      (update_low u n)
+      (fun _ s => LoopInv u (done_after done v) s).
+  Proof.
+    unfold LoopInv, LoopCoreInv.
+    apply Hoare_conj with
+      (Q1 := fun _ s => LoopAuxFacts u s).
+    { eapply Hoare_conseq_pre.
+      2: apply update_low_preserves_loop_aux_facts.
+      intros s [[Haux _] _]. exact Haux. }
+    apply Hoare_conj with
+      (Q1 := fun _ s => LoopCoreShape u (done_after done v) s).
+    { eapply Hoare_conseq_pre.
+      2: apply update_low_active_direct_preserves_loop_core_shape.
+      intros s [[_ [Hshape _]] [Hedge [_ [Hvis _]]]].
+      exact (conj Hshape (conj Hedge Hvis)). }
+    apply Hoare_conj with
+      (Q1 := fun _ s => Closed s).
+    { eapply Hoare_conseq_pre.
+      2: apply update_low_preserves_closed.
+      intros s [[_ [_ [Hclosed _]]] _]. exact Hclosed. }
+    { eapply Hoare_conseq_pre.
+      2: apply update_low_active_direct_preserves_low_correct.
+      intros s [[_ [Hshape [_ Hlow]]] [Hedge [Hnot_done [Hvis [Hactive [Hnot_tree Hn]]]]]].
+      exact (conj Hshape
+              (conj Hlow
+                (conj Hedge
+                  (conj Hnot_done
+                    (conj Hvis
+                      (conj Hactive
+                        (conj Hnot_tree Hn))))))). }
+  Qed.
+
+  Lemma visited_active_branch_preserves_loop_inv
+        (u v: V) (done: V -> Prop):
+    Hoare
+      (fun s: St =>
+         LoopInv u done s /\
+         Edge u v /\
+         ~ done v /\
+         Visited v s /\
+         Active v s)
+      (dv <- get' (fun s => dfn s v);; update_low u dv)
+      (fun _ s => LoopInv u (done_after done v) s).
+  Proof.
+    intro_state.
+    eapply Hoare_bind. { eapply Hoare_get'. } simpl. intros dv.
+    eapply Hoare_conseq_pre.
+    2: apply update_low_active_direct_preserves_loop_inv.
+    intros s1 [Hs1 Hdv]. subst s1.
+    destruct H as [Hinv [Hedge [Hnot_done [Hvis Hactive]]]].
+    assert (Hnot_tree: ~ tree_edge s0 u v).
+    { eapply current_active_edge_not_tree; eauto. }
+    exact (conj Hinv
+            (conj Hedge
+              (conj Hnot_done
+                (conj Hvis
+                  (conj Hactive
+                    (conj Hnot_tree Hdv)))))).
+  Qed.
+
+  Lemma tree_reachable_to_graph_reachable (s: St) (x y: V):
+    TreeEdgesAreGraphEdges s ->
+    dg_reachable (state_to_dfs_tree g s root) x y ->
+    dg_reachable g x y.
+  Proof.
+    intros Htree_sound Hreach.
+    eapply dg_reachable_lift.
+    - intros a b Hstep.
+      apply Htree_sound. exact Hstep.
+    - exact Hreach.
+  Qed.
+
+  Lemma inactive_done_no_new_target
+        (u v b: V) (done: V -> Prop) (s: St):
+    Closed s ->
+    TreeEdgesAreGraphEdges s ->
+    Visited v s ->
+    ~ Active v s ->
+    Edge u v ->
+    PartialLowCandidate u (done_after done v) s b ->
+    PartialLowCandidate u done s b.
+  Proof.
+    intros Hclosed Htree_sound Hvis Hnot_active _ Hcandidate.
+    unfold PartialLowCandidate in Hcandidate |- *.
+    destruct Hcandidate as [Hb_root | Htarget].
+    - left. exact Hb_root.
+    - unfold PartialActiveTarget in Htarget |- *.
+      destruct Htarget as [Hdirect | Hchild].
+      + destruct Hdirect as [a [Hdone_after [Hb [Hedge [Hactive Hnot_tree]]]]].
+        destruct (done_after_elim done v a Hdone_after) as [Hdone | Ha_eq_v].
+        * right. left. exists a. repeat split; auto.
+        * exfalso. apply Hnot_active.
+          rewrite Ha_eq_v in Hactive. exact Hactive.
+      + destruct Hchild as
+          [child [x [Hdone_after [Hedge [Hfa [Hfane [Hreach [Hxb [Hactive Hnot_tree]]]]]]]]].
+        destruct (done_after_elim done v child Hdone_after) as [Hdone | Hchild_eq_v].
+        * right. right. exists child, x. repeat split; auto.
+        * exfalso.
+          rewrite Hchild_eq_v in Hreach.
+          assert (Htree_graph: dg_reachable g v x).
+          { eapply tree_reachable_to_graph_reachable; eauto. }
+          assert (Hreach_target: dg_reachable g v b).
+          { eapply dg_reachable_step_reachable; eauto. }
+          exact (Hclosed v b Hvis Hnot_active Hreach_target Hactive).
+  Qed.
+
+  Lemma low_correct_add_inactive_done
+        (u v: V) (done: V -> Prop) (s: St):
+    Closed s ->
+    TreeEdgesAreGraphEdges s ->
+    Visited v s ->
+    ~ Active v s ->
+    Edge u v ->
+    LowCorrect u done s ->
+    LowCorrect u (done_after done v) s.
+  Proof.
+    intros Hclosed Htree_sound Hvis Hnot_active Hedge [Hsound Hcomplete].
+    split.
+    - destruct Hsound as [witness [Hcandidate Hlow]].
+      exists witness. split.
+      + apply partial_low_candidate_done_mono. exact Hcandidate.
+      + exact Hlow.
+    - intros target Hcandidate.
+      apply Hcomplete.
+      eapply inactive_done_no_new_target; eauto.
+  Qed.
+
+  Lemma visited_inactive_branch_preserves_loop_inv
+        (u v: V) (done: V -> Prop):
+    Hoare
+      (fun s: St =>
+         LoopInv u done s /\
+         Edge u v /\
+         ~ done v /\
+         Visited v s /\
+         ~ Active v s)
+      (ret tt)
+      (fun _ s => LoopInv u (done_after done v) s).
+  Proof.
+    unfold Hoare, ret. simpl. sets_unfold.
+    unfold StateRelMonad.ret.
+    intros s1 retv s2 Hpre [Hret Hstate].
+    subst retv s2.
+    destruct Hpre as [Hinv [Hedge [_ [Hvis Hnot_active]]]].
+    destruct Hinv as [Haux [Hshape [Hclosed Hlow]]].
+    destruct Hshape as [Hwf [Htree_sound [Huvis [Hdone_edge [Hdone_vis Hprocessed]]]]].
+    assert (Hshape_old: LoopCoreShape u done s1).
+    { exact (conj Hwf
+              (conj Htree_sound
+                (conj Huvis
+                  (conj Hdone_edge
+                    (conj Hdone_vis Hprocessed))))). }
+    unfold LoopInv, LoopCoreInv.
+    split.
+    - exact Haux.
+    - split.
+      + apply loop_core_shape_done_after_active; auto.
+      + split.
+        * exact Hclosed.
+        * apply low_correct_add_inactive_done; auto.
+  Qed.
+
+  Lemma tree_reachable_from_root_cases (s: St) (v x: V):
+    TreeEdgesAreGraphEdges s ->
+    dg_reachable (state_to_dfs_tree g s root) v x ->
+    x = v \/
+    exists child,
+      Edge v child /\
+      fa s child = v /\
+      fa s child <> child /\
+      dg_reachable (state_to_dfs_tree g s root) child x.
+  Proof.
+    intros Htree_sound Hreach.
+    unfold dg_reachable in Hreach.
+    induction Hreach as [a b Hstep | a | a b c Hreach_ab IH_ab Hreach_bc IH_bc].
+    - right. exists b.
+      pose proof Hstep as Hstep_tree.
+      apply tree_step_char in Hstep_tree as [Hfa [Hfane _]].
+      split.
+      + apply Htree_sound. exact Hstep.
+      + split; [exact Hfa | split; [exact Hfane |]].
+        unfold dg_reachable.
+        apply Coq.Relations.Relation_Operators.rt_refl.
+    - left. reflexivity.
+    - destruct IH_ab as [Hb_eq | [child [Hedge [Hfa [Hfane Hreach_child_b]]]]].
+      + subst b. exact IH_bc.
+      + right. exists child. repeat split; auto.
+        eapply dg_reachable_trans; eauto.
+  Qed.
+
+  Lemma tree_escape_to_child_candidate
+        (v x b: V) (s: St):
+    TreeEdgesAreGraphEdges s ->
+    dg_reachable (state_to_dfs_tree g s root) v x ->
+    Edge x b ->
+    Active b s ->
+    ~ tree_edge s x b ->
+    PartialLowCandidate v (edge_set v) s b.
+  Proof.
+    intros Htree_sound Hreach Hedge Hactive Hnot_tree.
+    destruct (tree_reachable_from_root_cases s v x Htree_sound Hreach)
+      as [Hx_eq_v | [child [Hchild_edge [Hfa [Hfane Hreach_child_x]]]]].
+    - subst x. right. left.
+      exists b. repeat split; auto.
+    - right. right.
+      exists child, x. repeat split; auto.
+  Qed.
+
+  Lemma child_candidate_lifts_to_parent
+        (u v b: V) (done: V -> Prop) (s: St):
+    LoopCoreShape v (edge_set v) s ->
+    Edge u v ->
+    fa s v = u ->
+    fa s v <> v ->
+    PartialLowCandidate v (edge_set v) s b ->
+    b = v \/ PartialActiveTarget u (done_after done v) s b.
+  Proof.
+    intros Hshape Hedge_uv Hfa_v Hfane_v Hcandidate.
+    destruct Hcandidate as [Hb_eq_v | Htarget].
+    - left. exact Hb_eq_v.
+    - right.
+      destruct Hshape as [_ [_ [_ [_ [Hdone_vis _]]]]].
+      unfold PartialActiveTarget in Htarget |- *.
+      destruct Htarget as [Hdirect | Hchild].
+      + destruct Hdirect as [a [Hdone [Hb [Hedge [Hactive Hnot_tree]]]]].
+        right. exists v, v.
+        repeat split; auto.
+        * apply done_after_intro_new.
+        * unfold dg_reachable.
+          apply Coq.Relations.Relation_Operators.rt_refl.
+        * rewrite Hb. exact Hedge.
+        * rewrite Hb. exact Hactive.
+        * rewrite Hb. exact Hnot_tree.
+      + destruct Hchild as
+          [child [x [Hdone [Hedge [Hfa [Hfane [Hreach [Hxb [Hactive Hnot_tree]]]]]]]]].
+        assert (Hchild_vis: Visited child s).
+        { apply Hdone_vis. exact Hdone. }
+        assert (Htree_v_child: tree_edge s v child).
+        { unfold tree_edge.
+          eapply tree_step_char_backward; eauto. }
+        assert (Hreach_v_x:
+                  dg_reachable (state_to_dfs_tree g s root) v x).
+        { eapply dg_step_reachable_reachable; eauto. }
+        right. exists v, x.
+        repeat split; auto.
+        apply done_after_intro_new.
+  Qed.
+
+  Lemma parent_candidate_done_after_child_cases
+        (u v b: V) (done: V -> Prop) (s: St):
+    TreeEdgesAreGraphEdges s ->
+    Edge u v ->
+    Visited v s ->
+    fa s v = u ->
+    fa s v <> v ->
+    PartialLowCandidate u (done_after done v) s b ->
+    PartialLowCandidate u done s b \/
+    exists x,
+      dg_reachable (state_to_dfs_tree g s root) v x /\
+      Edge x b /\
+      Active b s /\
+      ~ tree_edge s x b.
+  Proof.
+    intros _ Hedge_uv Hvis_v Hfa_v Hfane_v Hcandidate.
+    assert (Htree_uv: tree_edge s u v).
+    { unfold tree_edge.
+      eapply tree_step_char_backward; eauto. }
+    unfold PartialLowCandidate in Hcandidate |- *.
+    destruct Hcandidate as [Hb_root | Htarget].
+    - left. left. exact Hb_root.
+    - unfold PartialActiveTarget in Htarget |- *.
+      destruct Htarget as [Hdirect | Hchild].
+      + destruct Hdirect as [a [Hdone_after [Hb [Hedge [Hactive Hnot_tree]]]]].
+        destruct (done_after_elim done v a Hdone_after) as [Hdone | Ha_eq_v].
+        * left. right. left.
+          exists a. repeat split; auto.
+        * subst a. subst b.
+          exfalso. apply Hnot_tree. exact Htree_uv.
+      + destruct Hchild as
+          [child [x [Hdone_after [Hedge [Hfa [Hfane [Hreach [Hxb [Hactive Hnot_tree]]]]]]]]].
+        destruct (done_after_elim done v child Hdone_after) as [Hdone | Hchild_eq_v].
+        * left. right. right.
+          exists child, x. repeat split; auto.
+        * subst child. right.
+          exists x. repeat split; auto.
+  Qed.
+
+  Lemma low_correct_add_child_contribution_value
+        (u v: V) (done: V -> Prop) (s_before s: St) (n: nat):
+    LoopInv u done s_before ->
+    Edge u v ->
+    ParentLowFrame u done s_before s ->
+    TreeEdgesAreGraphEdges s ->
+    Visited v s ->
+    fa s v = u ->
+    fa s v <> v ->
+    ChildLowContribution u v s ->
+    n = Nat.min (low s_before u) (low s v) ->
+    (exists witness,
+       PartialLowCandidate u (done_after done v) s witness /\
+       n = dfn s witness) /\
+    (forall target,
+       PartialLowCandidate u (done_after done v) s target ->
+       n <= dfn s target).
+  Proof.
+    intros Hinv Hedge_uv Hframe Htree_sound Hvis_v Hfa_v Hfane_v
+           Hchild_contrib Hn.
+    destruct Hinv as [_ [_ [_ [Hsound_old Hcomplete_old]]]].
+    destruct Hframe as [_ [Hframe_fwd Hframe_bwd]].
+    assert (Hroot_before: PartialLowCandidate u done s_before u).
+    { apply partial_low_candidate_root. }
+    pose proof (Hcomplete_old u Hroot_before) as Hlow_before_le_dfn_before_u.
+    destruct (Hframe_fwd u Hroot_before) as [_ Hdfn_u_eq].
+    assert (Hlow_before_le_dfn_u: low s_before u <= dfn s u) by lia.
+    split.
+    - destruct (Nat.le_gt_cases (low s_before u) (low s v))
+        as [Hold_le | Hchild_lt].
+      + destruct Hsound_old as [witness [Hcandidate_before Hlow_before_eq]].
+        destruct (Hframe_fwd witness Hcandidate_before) as
+          [Hcandidate_after Hdfn_w_eq].
+        exists witness. split.
+        * apply partial_low_candidate_done_mono. exact Hcandidate_after.
+        * subst n. rewrite Nat.min_l by exact Hold_le. lia.
+      + destruct Hchild_contrib as
+          [[Hv_active [Hchild_shape [Hchild_sound _]]] |
+           [Hv_inactive [Hlow_v_eq [Hdfn_lt Hno_target]]]].
+        * destruct Hchild_sound as [witness [Hcandidate_child Hlow_v_witness]].
+          destruct (child_candidate_lifts_to_parent
+                      u v witness done s Hchild_shape Hedge_uv Hfa_v
+                      Hfane_v Hcandidate_child)
+            as [Hwitness_eq_v | Hparent_target].
+          -- subst witness.
+             destruct Hchild_shape as [Hwf_child _].
+             destruct Hwf_child as [_ [_ [Hdfn_valid _]]].
+             assert (Hdfn_parent_child: dfn s u < dfn s v).
+             { eapply fa_parent_dfn_lt; eauto. }
+             lia.
+          -- exists witness. split.
+             ++ right. exact Hparent_target.
+             ++ subst n. rewrite Nat.min_r by lia. lia.
+        * lia.
+    - intros target Hcandidate_after.
+      subst n.
+      destruct (parent_candidate_done_after_child_cases
+                  u v target done s Htree_sound Hedge_uv Hvis_v
+                  Hfa_v Hfane_v Hcandidate_after)
+        as [Hcandidate_old_after |
+            [x [Hreach_v_x [Hedge_x_target [Hactive_target Hnot_tree]]]]].
+      + destruct (Hframe_bwd target Hcandidate_old_after) as
+          [Hcandidate_before Hdfn_target_eq].
+        pose proof (Hcomplete_old target Hcandidate_before) as Hcomplete_target.
+        pose proof (Nat.le_min_l (low s_before u) (low s v)) as Hmin_le_old.
+        lia.
+      + destruct Hchild_contrib as
+          [[Hv_active [Hchild_shape [_ Hchild_complete]]] |
+           [Hv_inactive [Hlow_v_eq [Hdfn_lt Hno_target]]]].
+        * assert (Hcandidate_child:
+                    PartialLowCandidate v (edge_set v) s target).
+          { eapply tree_escape_to_child_candidate; eauto. }
+          pose proof (Hchild_complete target Hcandidate_child)
+            as Hchild_complete_target.
+          pose proof (Nat.le_min_r (low s_before u) (low s v)) as Hmin_le_child.
+          lia.
+        * exfalso.
+          exact (Hno_target x target Hreach_v_x Hedge_x_target
+                            Hactive_target Hnot_tree).
+  Qed.
+
+  Lemma update_low_child_contribution_preserves_low_correct
+        (u v: V) (done: V -> Prop) (s_before: St) (n: nat):
+    Hoare
+      (fun s: St =>
+         LoopInv u done s_before /\
+         Edge u v /\
+         ChildContributionContract u v done s_before s /\
+         n = low s v)
+      (update_low u n)
+      (fun _ s => LowCorrect u (done_after done v) s).
+  Proof.
+    unfold update_low. unfold_op. intro_state. hoare_auto_s.
+    - subst s. simpl.
+      destruct H as [Hinv [Hedge_uv [Hcontract Hn_low_v]]].
+      destruct Hcontract as
+        [Hframe [Hshape [Haux [Hclosed [Htree [Hvis [Hfa [Hfane Hchild]]]]]]]].
+      destruct Hframe as [Hlow_u_frame Hframe_rest].
+      assert (Hframe_all:
+                ParentLowFrame u done s_before s0).
+      { exact (conj Hlow_u_frame Hframe_rest). }
+      assert (Hn_min:
+                n = Nat.min (low s_before u) (low s0 v)).
+      { rewrite <- Hlow_u_frame.
+        rewrite <- Hn_low_v.
+        rewrite Nat.min_r by lia.
+        reflexivity. }
+      destruct (low_correct_add_child_contribution_value
+                  u v done s_before s0 n Hinv Hedge_uv Hframe_all
+                  Htree Hvis Hfa Hfane Hchild Hn_min)
+        as [Hsound_value Hcomplete_value].
+      split.
+      + destruct Hsound_value as [witness [Hcandidate Hlow_witness]].
+        exists witness. split.
+        * change (PartialLowCandidate u (done_after done v) s0 witness).
+          exact Hcandidate.
+        * simpl. unfold equiv_decb.
+          destruct (equiv_dec u u) as [_ | Hneq].
+          -- exact Hlow_witness.
+          -- exfalso. apply Hneq. reflexivity.
+      + intros target Hcandidate.
+        simpl. unfold equiv_decb.
+        destruct (equiv_dec u u) as [_ | Hneq].
+        * apply Hcomplete_value.
+          change (PartialLowCandidate u (done_after done v) s0 target)
+            in Hcandidate.
+          exact Hcandidate.
+        * exfalso. apply Hneq. reflexivity.
+    - destruct H1 as [Heq Hnot_lt]. subst s.
+      destruct H as [Hinv [Hedge_uv [Hcontract Hn_low_v]]].
+      destruct Hcontract as
+        [Hframe [Hshape [Haux [Hclosed [Htree [Hvis [Hfa [Hfane Hchild]]]]]]]].
+      destruct Hframe as [Hlow_u_frame Hframe_rest].
+      assert (Hframe_all:
+                ParentLowFrame u done s_before s0).
+      { exact (conj Hlow_u_frame Hframe_rest). }
+      assert (Hn_min:
+                low s0 u = Nat.min (low s_before u) (low s0 v)).
+      { rewrite <- Hlow_u_frame.
+        rewrite <- Hn_low_v.
+        rewrite Nat.min_l by lia.
+        reflexivity. }
+      destruct (low_correct_add_child_contribution_value
+                  u v done s_before s0 (low s0 u) Hinv Hedge_uv Hframe_all
+                  Htree Hvis Hfa Hfane Hchild Hn_min)
+        as [Hsound_value Hcomplete_value].
+      exact (conj Hsound_value Hcomplete_value).
+  Qed.
+
+  Lemma update_low_child_contribution_preserves_loop_core_shape
+        (u v: V) (done: V -> Prop) (s_before: St) (n: nat):
+    Hoare
+      (fun s: St =>
+         ChildContributionContract u v done s_before s)
+      (update_low u n)
+      (fun _ s => LoopCoreShape u (done_after done v) s).
+  Proof.
+    eapply Hoare_conseq_pre.
+    2: apply update_low_preserves_loop_core_shape.
+    intros s Hcontract.
+    destruct Hcontract as [_ [Hshape _]].
+    pose proof Hshape as Hshape_copy.
+    destruct Hshape_copy as [_ [_ [Huvis _]]].
+    exact (conj Hshape Huvis).
+  Qed.
+
+  Lemma update_low_child_contribution_preserves_loop_inv
+        (u v: V) (done: V -> Prop) (s_before: St) (n: nat):
+    Hoare
+      (fun s: St =>
+         LoopInv u done s_before /\
+         Edge u v /\
+         ChildContributionContract u v done s_before s /\
+         n = low s v)
+      (update_low u n)
+      (fun _ s => LoopInv u (done_after done v) s).
+  Proof.
+    unfold LoopInv, LoopCoreInv.
+    apply Hoare_conj with
+      (Q1 := fun _ s => LoopAuxFacts u s).
+    { eapply Hoare_conseq_pre.
+      2: apply update_low_preserves_loop_aux_facts.
+      intros s [_ [_ [Hcontract _]]].
+      destruct Hcontract as [_ [_ [Haux _]]].
+      exact Haux. }
+    apply Hoare_conj with
+      (Q1 := fun _ s => LoopCoreShape u (done_after done v) s).
+    { eapply Hoare_conseq_pre.
+      2: apply update_low_child_contribution_preserves_loop_core_shape.
+      intros s [_ [Hedge [Hcontract _]]].
+      exact Hcontract. }
+    apply Hoare_conj with
+      (Q1 := fun _ s => Closed s).
+    { eapply Hoare_conseq_pre.
+      2: apply update_low_preserves_closed.
+      intros s [_ [_ [Hcontract _]]].
+      destruct Hcontract as [_ [_ [_ [Hclosed _]]]].
+      exact Hclosed. }
+    { eapply Hoare_conseq_pre.
+      2: apply update_low_child_contribution_preserves_low_correct.
+      intros s [Hinv [Hedge [Hcontract Hn]]].
+      exact (conj Hinv (conj Hedge (conj Hcontract Hn))). }
+  Qed.
+
+  Lemma get_low_update_low_child_contribution_preserves_loop_inv
+        (u v: V) (done: V -> Prop) (s_before: St):
+    Hoare
+      (fun s: St =>
+         LoopInv u done s_before /\
+         Edge u v /\
+         ChildContributionContract u v done s_before s)
+      (lv <- get' (fun s => low s v);; update_low u lv)
+      (fun _ s => LoopInv u (done_after done v) s).
+  Proof.
+    intro_state.
+    eapply Hoare_bind. { eapply Hoare_get'. } simpl. intros lv.
+    eapply Hoare_conseq_pre.
+    2: apply update_low_child_contribution_preserves_loop_inv.
+    intros s1 [Hs1 Hlv]. subst s1.
+    destruct H as [Hinv [Hedge Hcontract]].
+    exact (conj Hinv (conj Hedge (conj Hcontract Hlv))).
+  Qed.
+
+  Lemma get_low_update_low_child_contribution_preserves_loop_inv_exists
+        (u v: V) (done: V -> Prop):
+    Hoare
+      (fun s: St =>
+         exists s_before,
+           LoopInv u done s_before /\
+           Edge u v /\
+           ChildContributionContract u v done s_before s)
+      (lv <- get' (fun s => low s v);; update_low u lv)
+      (fun _ s => LoopInv u (done_after done v) s).
+  Proof.
+    unfold Hoare.
+    intros s1 retv s2 [s_before Hpre] Hexec.
+    pose proof
+      (get_low_update_low_child_contribution_preserves_loop_inv
+         u v done s_before) as Hhoare.
+    unfold Hoare in Hhoare.
+    exact (Hhoare s1 retv s2 Hpre Hexec).
+  Qed.
+
+  Lemma unvisited_tree_child_branch_preserves_loop_inv
+        (u v: V) (done: V -> Prop) (W: RecProgram):
+    Hoare
+      (fun s: St =>
+         LoopInv u done s /\
+         Edge u v /\
+         EntryPre v s /\
+         fa s v = u /\
+         fa s v <> v)
+      (W v)
+      (fun _ s =>
+         exists s_before,
+           LoopInv u done s_before /\
+           Edge u v /\
+           ChildContributionContract u v done s_before s) ->
+    Hoare
+      (fun s: St =>
+         LoopInv u done s /\
+         Edge u v /\
+         ~ Visited v s)
+      (set_fa v u;;
+       W v;;
+       lv <- get' (fun s => low s v);;
+       update_low u lv)
+      (fun _ s => LoopInv u (done_after done v) s).
+  Proof.
+    intros HW.
+    eapply Hoare_bind.
+    { apply set_fa_pending_prepares_child_entry. }
+    simpl. intros _.
+    eapply Hoare_bind.
+    { eapply Hoare_conseq_pre.
+      2: exact HW.
+      intros s [Hloop [Hentry [Hfa Hfane]]].
+      assert (Hedge: Edge u v).
+      { destruct Hentry as [_ [_ [_ [_ [_ Hincoming]]]]].
+        rewrite <- Hfa. apply Hincoming. exact Hfane. }
+      exact (conj Hloop
+              (conj Hedge
+                (conj Hentry
+                  (conj Hfa Hfane)))). }
+    simpl. intros _.
+    apply get_low_update_low_child_contribution_preserves_loop_inv_exists.
+  Qed.
+
+  Lemma process_edge_preserves_loop_inv
+        (u v: V) (done: V -> Prop) (W: RecProgram):
+    Hoare
+      (fun s: St =>
+         LoopInv u done s /\
+         Edge u v /\
+         EntryPre v s /\
+         fa s v = u /\
+         fa s v <> v)
+      (W v)
+      (fun _ s =>
+         exists s_before,
+           LoopInv u done s_before /\
+           Edge u v /\
+           ChildContributionContract u v done s_before s) ->
+    Hoare
+      (fun s: St =>
+         LoopInv u done s /\
+         Edge u v /\
+         ~ done v)
+      (process_edge u W v)
+      (fun _ s => LoopInv u (done_after done v) s).
+  Proof.
+    intros HW.
+    unfold process_edge, if_else.
+    intro_state.
+    apply Hoare_choice.
+    - apply Hoare_assume_bind. simpl.
+      eapply Hoare_conseq_pre.
+      2: apply (unvisited_tree_child_branch_preserves_loop_inv
+                  u v done W HW).
+      intros s1 [Hnotvis Hs1]. subst s1.
+      destruct H as [Hinv [Hedge _]].
+      exact (conj Hinv (conj Hedge Hnotvis)).
+    - apply Hoare_assume_bind. simpl.
+      intro_state.
+      destruct H1 as [Hvisited_by_classic Hs1]. subst s1.
+      apply Hoare_choice.
+      + apply Hoare_assume_bind. simpl.
+        eapply Hoare_conseq_pre.
+        2: apply visited_active_branch_preserves_loop_inv.
+        intros s1 [Hactive Hs1]. subst s1.
+        destruct H as [Hinv [Hedge Hnotdone]].
+        assert (Hvis: Visited v s0).
+        { unfold Visited. apply NNPP. exact Hvisited_by_classic. }
+        assert (Hactive': Active v s0).
+        { unfold Active. exact Hactive. }
+        exact (conj Hinv
+                (conj Hedge
+                  (conj Hnotdone
+                    (conj Hvis Hactive')))).
+      + eapply Hoare_conseq_post.
+        2: { apply Hoare_assume_s. }
+        simpl. intros _ s [Heq Hnotactive]. subst s.
+        destruct H as [Hinv [Hedge _]].
+        assert (Hvis: Visited v s0).
+        { unfold Visited. apply NNPP. exact Hvisited_by_classic. }
+        assert (Hnotactive': ~ Active v s0).
+        { unfold Active. exact Hnotactive. }
+        destruct Hinv as [Haux [Hshape [Hclosed Hlow]]].
+        pose proof Hshape as Hshape_old.
+        destruct Hshape as
+          [Hwf [Htree_sound [Huvis [Hdone_edge [Hdone_vis Hprocessed]]]]].
+        unfold LoopInv, LoopCoreInv.
+        split; [exact Haux |].
+        split.
+        * apply loop_core_shape_done_after_active; auto.
+        * split; [exact Hclosed |].
+          apply low_correct_add_inactive_done; auto.
+  Qed.
+
+  Lemma process_edge_preserves_stack_nodup
+        (u v: V) (W: RecProgram):
+    (forall x, Hoare StackNoDup (W x) (fun _ s => StackNoDup s)) ->
+    Hoare StackNoDup
+          (process_edge u W v)
+          (fun _ s => StackNoDup s).
+  Proof.
+    intros HW.
+    unfold process_edge, if_else.
+    intro_state.
+    apply Hoare_choice.
+    - apply Hoare_assume_bind. simpl.
+      apply Hoare_conseq_pre with (P2 := StackNoDup).
+      intros s1 [_ Hs1]. subst s1. exact H.
+      hoare_bind (set_fa_preserves_stack_nodup v u). simpl. clear a.
+      eapply Hoare_bind.
+      { apply HW. }
+      simpl. intros _.
+      apply get_low_update_low_preserves_stack_nodup.
+    - intro_state. hoare_auto_s.
+      + eapply Hoare_conseq_pre.
+        2: apply (update_low_preserves_stack_nodup u (dfn s0 v)).
+        intros s1 Hs1. subst s1. exact H.
+      + destruct H3 as [Heq _]. subst s. subst s1. exact H.
+  Qed.
+
+  Lemma process_edge_preserves_loop_aux_facts
+        (u v: V) (W: RecProgram):
+    (forall x,
+       Hoare NoUnvisitedReach (W x) (fun _ s => NoUnvisitedReach s)) ->
+    (forall x,
+       Hoare (Active u) (W x) (fun _ s => Active u s)) ->
+    (forall x,
+       Hoare stack_dfn_order (W x) (fun _ s => stack_dfn_order s)) ->
+    (forall x,
+       Hoare dfn_injective (W x) (fun _ s => dfn_injective s)) ->
+    (forall x,
+       Hoare StackNoDup (W x) (fun _ s => StackNoDup s)) ->
+    Hoare (LoopAuxFacts u)
+          (process_edge u W v)
+          (fun _ s => LoopAuxFacts u s).
+  Proof.
+    intros HWsettled HWactive HWorder HWinj HWnodup.
+    unfold LoopAuxFacts, OrderFacts.
+    apply Hoare_conj with
+      (Q1 := fun _ s => NoUnvisitedReach s).
+    { eapply Hoare_conseq_pre.
+      2: { apply process_edge_keep_settled_closed.
+           intros x. apply HWsettled. }
+      intros s [Hsettled _]. exact Hsettled. }
+    apply Hoare_conj with
+      (Q1 := fun _ s => Active u s).
+    { eapply Hoare_conseq_pre.
+      2: { apply process_edge_keep_in_stack.
+           intros x. apply HWactive. }
+      intros s [_ [Hactive _]]. exact Hactive. }
+    apply Hoare_conj with
+      (Q1 := fun _ s => stack_dfn_order s).
+    { eapply Hoare_conseq_pre.
+      2: { apply process_edge_preserves_stack_dfn_order.
+           intros x. apply HWorder. }
+      intros s [_ [_ [Hstack_order _]]]. exact Hstack_order. }
+    apply Hoare_conj with
+      (Q1 := fun _ s => dfn_injective s).
+    { eapply Hoare_conseq_pre.
+      2: { apply process_edge_keep_dfn_injective.
+           intros x. apply HWinj. }
+      intros s [_ [_ [_ [Hinj _]]]]. exact Hinj. }
+    { eapply Hoare_conseq_pre.
+      2: { apply process_edge_preserves_stack_nodup.
+           intros x. apply HWnodup. }
+      intros s [_ [_ [_ [_ Hnodup]]]]. exact Hnodup. }
+  Qed.
+
+  Lemma forset_process_edge_preserves_loop_aux_facts
+        (u: V) (W: RecProgram):
+    (forall x,
+       Hoare NoUnvisitedReach (W x) (fun _ s => NoUnvisitedReach s)) ->
+    (forall x,
+       Hoare (Active u) (W x) (fun _ s => Active u s)) ->
+    (forall x,
+       Hoare stack_dfn_order (W x) (fun _ s => stack_dfn_order s)) ->
+    (forall x,
+       Hoare dfn_injective (W x) (fun _ s => dfn_injective s)) ->
+    (forall x,
+       Hoare StackNoDup (W x) (fun _ s => StackNoDup s)) ->
+    Hoare (LoopAuxFacts u)
+          (forset (fun v => dg_step g u v) (process_edge u W))
+          (fun _ s => LoopAuxFacts u s).
+  Proof.
+    intros HWsettled HWactive HWorder HWinj HWnodup.
+    unfold forset. hoare_fix_nolv_auto (V -> Prop).
+    simpl; intros W0 IH0 todo.
+    unfold forset_f. hoare_auto_s. intro_state. hoare_auto_s.
+    eapply Hoare_bind with (R := fun (_: unit) s => LoopAuxFacts u s).
+    { apply Hoare_conseq_pre with (P2 := LoopAuxFacts u).
+      { intros s1 Hs1. subst s1. exact H. }
+      apply process_edge_preserves_loop_aux_facts; auto. }
+    simpl. intros _. apply IH0.
+  Qed.
+
+  Lemma edge_loop_preserves_loop_inv
+        (u: V) (W: RecProgram):
+    (forall done v,
+       done ⊆ edge_set u ->
+       Edge u v ->
+       ~ done v ->
+       Hoare
+         (fun s: St =>
+            LoopInv u done s /\
+            Edge u v /\
+            EntryPre v s /\
+            fa s v = u /\
+            fa s v <> v)
+         (W v)
+         (fun _ s =>
+            exists s_before,
+              LoopInv u done s_before /\
+              Edge u v /\
+              ChildContributionContract u v done s_before s)) ->
+    Hoare
+      (fun s: St => LoopInv u ∅ s)
+      (forset (edge_set u) (process_edge u W))
+      (fun _ s => LoopInv u (edge_set u) s).
+  Proof.
+    intros HW.
+    apply Hoare_forset with
+      (P := fun done s => LoopInv u done s)
+      (universe := edge_set u).
+    - intros done1 done2 Hdone s1 s2 Heq. subst s2.
+      split; intro Hinv.
+      + eapply loop_inv_done_equiv; eauto.
+      + eapply loop_inv_done_equiv.
+        * symmetry. exact Hdone.
+        * exact Hinv.
+    - intros done a Hdone_sub Hedge Hnot_done.
+      eapply Hoare_conseq_pre.
+      2: {
+        eapply process_edge_preserves_loop_inv.
+        apply HW; auto. }
+      intros s Hinv.
+      exact (conj Hinv (conj Hedge Hnot_done)).
+  Qed.
+
+  (* maybe pop *)
+  
 End IS_LOW.
